

# Numerics for PDEs

## (1) BS-PDE:

Consider BS model:  $dS_t/S_t = r dt + \sigma dB_t$ .  $S_0 = s$ .

$\Rightarrow$  price  $u(t, x) = \mathbb{E}(e^{-r(\tau-t)} f(S_\tau) | S_t = x)$  of payoff  $f$  on European option will satisfy

BS-PDE (also parabolic PDE):

$$\begin{cases} \frac{\partial}{\partial t} u(t, x) + \frac{1}{2} \sigma^2 x^2 \frac{\partial^2}{\partial x^2} u(t, x) + rx \frac{\partial}{\partial x} u(t, x) = ru(t, x) \\ u(T, x) = f(x). \end{cases}$$

For American option, price  $\tilde{u}$  satisfies:

$$(6.2a) \quad \frac{\partial}{\partial t} \tilde{u}(t, x) + \frac{1}{2} \sigma^2 x^2 \frac{\partial^2}{\partial x^2} \tilde{u}(t, x) + rx \frac{\partial}{\partial x} \tilde{u}(t, x) - r\tilde{u}(t, x) \leq 0,$$

$$(6.2b) \quad \tilde{u}(t, x) \geq (K - x)_+,$$

$$(6.2c) \quad \tilde{u}(T, x) = (K - x)_+,$$

Remark: We have equality in (6.2a) if ineq. in (6.2b) is strict. It's a free boundary problem. i.e.  $\exists X_*(t)$  st.  $\tilde{u}$  solves (6.2a) with equality on  $(X_*(t), \infty)$  (behaves like European option). And  $\tilde{u}(t, x) = (K - X_*(t))_+$  else.

To solve the two problems numerically. We first need to simplify the PDEs:

Let  $y = \log(x/k)$ .  $z = \frac{1}{2} \sigma^2 (T-t)$ .  $\eta = 2\sqrt{\tau}/\sigma^2$

$$V(z, \eta) = \frac{1}{k} \exp\left(\frac{1}{2}(\eta-1)\eta + \left(\frac{1}{4}(\eta-1)^2 + \eta\right)z\right) u(t, x)$$

and denote  $\tilde{V}$  for  $\tilde{u}$  in same way.

Prop:  $V(z, \eta) \rightarrow \exp\left(\frac{1}{2}(\eta-1)\eta + \frac{1}{4}(\eta-1)^2 z\right) \quad (\eta \rightarrow -\infty)$

$$V(z, \eta) \rightarrow 0 \quad (\eta \rightarrow +\infty).$$

$$V \text{ satisfies: } \frac{\partial}{\partial z} V = \frac{\partial^2}{\partial \eta^2} V.$$

$$V(0, \eta) = \left( e^{\frac{1}{2}(\eta-1)\eta} - e^{\frac{1}{2}(\eta+1)\eta} \right)_+.$$

For American option:

let  $g(y, \tau) := \exp\left(\frac{1}{4}(q+1)^2 \tau\right) \left( e^{\frac{1}{2}(q-1)y} - e^{\frac{1}{2}(q+1)y} \right)_+$ , then

$$(6.6a) \quad \left( \frac{\partial}{\partial \tau} \tilde{v}(\tau, y) - \frac{\partial^2}{\partial y^2} \tilde{v}(\tau, y) \right) (\tilde{v}(\tau, y) - g(\tau, y)) = 0, \quad \frac{\partial}{\partial \tau} \tilde{v}(\tau, y) - \frac{\partial^2}{\partial y^2} \tilde{v}(\tau, y) \geq 0,$$

$$(6.6b) \quad \tilde{v}(\tau, y) \geq g(\tau, y), \quad \tilde{v}(0, y) = g(0, y),$$

$$(6.6c) \quad \tilde{v}(\tau, y) = g(\tau, y) \text{ for } y \rightarrow -\infty, \quad \tilde{v}(\tau, y) = 0 \text{ for } y \rightarrow \infty.$$

(2) Finite difference method:

Consider  $u(t, x)$  on  $[0, T] \times [a, b]$ . Let

$$\Delta t = \tau/N, \quad \Delta x = (b-a)/m, \quad t_i = i \Delta t, \quad x_j = a + j \Delta x.$$

$$V(t_i, x_j) := V_{i,j}, \quad 0 \leq i \leq N, \quad 0 \leq j \leq m.$$

mk: i) The limit behavior of  $V$  is necessary to set boundary value condition of  $V$  at  $x = a, b$ .

(e.g., let  $V(t, a) = V(t, -\infty)$ ,  $V(t, b) = V(t, +\infty)$ , for  $-a, b$  large)

ii) It still suffers curse of dim. since in  $\mathbb{R}^n$ . We need to set  $n$  nodes with same mesh  $\Delta x$ .

### ① Explicit case:

We use  $D_t^*$ ,  $D_x^2$  replace  $\partial/\partial t$ ,  $\partial^2/\partial x^2$ :

Denote  $\lambda := \Delta t / (\Delta x)^2$ . We have:

$$(6.9a) \quad v_{0,j} = \left( e^{\frac{1}{2}(q-1)x_j} - e^{\frac{1}{2}(q+1)x_j} \right)_+, \quad j = 0, \dots, M,$$

$$(6.9b) \quad v_{i+1,j} = v_{i,j} + \lambda(v_{i,j+1} - 2v_{i,j} + v_{i,j-1}), \quad i = 0, \dots, N-1, \quad j = 1, \dots, M-1,$$

$$(6.9c) \quad v_{i+1,0} = \exp\left(\frac{1}{2}(q-1)a + \frac{1}{4}(q-1)^2 t_{i+1}\right), \quad v_{i+1,M} = 0, \quad i = 0, \dots, N-1.$$

let  $V^{(i)} := (V_{i,1} \dots V_{i,m})$ . linear system:

$$(6.10) \quad v^{(i+1)} = A v^{(i)}, \quad A := \begin{pmatrix} 1-2\lambda & \lambda & 0 & \dots & 0 \\ \lambda & 1-2\lambda & \ddots & \ddots & \vdots \\ 0 & \ddots & \ddots & \ddots & 0 \\ \vdots & \ddots & \ddots & \ddots & \lambda \\ 0 & \dots & 0 & \lambda & 1-2\lambda \end{pmatrix}.$$

For the system to be stable:

Thm. If  $\Delta t \leq \frac{1}{2} (\Delta x)^2$ . Then the finite difference method is stable and converges with error  $= O(\Delta t) + O(\Delta x^2)$  if boundary cond. are exact.

Proof: Let  $N \sim n^2$ . Then error  $\sim n^{-2}$  and comp. cost  $\sim n^3$ .

If in  $n$ -dim. then the cost  $\sim n^{2+n}$ . (generally let  $n \leq 4$ ).

### ④ Implicit case:

Use  $D_t$ ,  $D_x^2$ :

$$V_{i+1,j} = V_{i,j} + \Delta t (-V_{i,j+1} + 2V_{i,j} - V_{i,j-1})$$

$$Av^{(i)} = v^{(i-1)}, \quad A := \begin{pmatrix} 1+2\lambda & -\lambda & 0 & \dots & 0 \\ -\lambda & 1+2\lambda & \ddots & \ddots & \vdots \\ 0 & \ddots & \ddots & \ddots & 0 \\ \vdots & \ddots & \ddots & \ddots & -\lambda \\ 0 & \dots & 0 & -\lambda & 1+2\lambda \end{pmatrix}.$$

Thm. It's uncond. stable for  $\Delta t > 0$  with error  $= O(\Delta t^2) + O(\Delta x^2)$  if BC is exact.

### ③ Crank - Nicolson:

use  $D_t^-(v_{i,j})$  and  $\frac{1}{2} (D_x^2(v_{i,j}) + D_x^2(v_{i+1,j}))$ :

$$\frac{v_{i+1,j} - v_{i,j}}{\Delta t} = \frac{1}{2\Delta x^2} (v_{i,j+1} - 2v_{i,j} + v_{i,j-1} + v_{i+1,j+1} - 2v_{i+1,j} + v_{i+1,j-1}).$$

And the linear system is:

(6.16)

$$Av^{(i+1)} = Bv^{(i)},$$

where

$$(6.17) \quad A := \begin{pmatrix} 1+\lambda & -\frac{\lambda}{2} & 0 & \dots & 0 \\ -\frac{\lambda}{2} & 1+\lambda & \ddots & \ddots & \vdots \\ 0 & \ddots & \ddots & \ddots & 0 \\ \vdots & \ddots & \ddots & \ddots & -\frac{\lambda}{2} \\ 0 & \dots & 0 & -\frac{\lambda}{2} & 1+\lambda \end{pmatrix}, B := \begin{pmatrix} 1-\lambda & \frac{\lambda}{2} & 0 & \dots & 0 \\ \frac{\lambda}{2} & 1-\lambda & \ddots & \ddots & \vdots \\ 0 & \ddots & \ddots & \ddots & 0 \\ \vdots & \ddots & \ddots & \ddots & \frac{\lambda}{2} \\ 0 & \dots & 0 & \frac{\lambda}{2} & 1-\lambda \end{pmatrix}$$

Thm. If the sol.  $u$  given  $B, C \in C^k$ . Then the method is stable for  $\forall \Delta x, \Delta t$  with error  $O(\Delta t^2) + O(\Delta x^2)$ .

### (3) Finite element method:

It's more applicable on time-independent PDEs.

Consider variation problem:  $A(u, v) = L(v)$  on  $V$

where  $A$  is sym. positive semidefinite bilinear form, i.e.  $A(v, v) \geq \alpha \|v\|_V^2$ ,  $|A(u, v)| \leq C \|u\|_V \|v\|_V$ ,

LEM. (minimization problem)

$u$  solves the variation problem  $(\Rightarrow u$  is minimizer of  $F(u) := \frac{1}{2} A(u, u) - L(u)$ )

Pf:  $(\Leftarrow) \forall v \in V$ . assume  $v = u + \varepsilon w$ .  $\varepsilon \in \mathbb{R}$ .

$$\text{Then: } F(v) = F(u + \varepsilon w) =: f(\varepsilon)$$

$$\frac{d}{d\varepsilon} f(\varepsilon) = 0 \Leftrightarrow A(u, w) = L(w). \forall w \in V.$$

$\Leftrightarrow u$  solves the problem.

$$(\Rightarrow) F(v) = F(u + \varepsilon w)$$

$$= \left( \frac{1}{2} A(u, u) - L(u) \right) + \varepsilon (A(u, w) - L(w)) + \frac{1}{2} \varepsilon^2 A(w, w) \geq F(u).$$

Remark: It offers a diff. method to prove Lax-Milgram Thm:  
let  $(v_n) \subset V$ .  $F(v_n) \rightarrow \inf_v F(v)$   
prove it's Cauchy

To apply FEM:

- 1) we derive its variation formulation by partial integrals on  $V$  ( $:= H_0^1$ )
- 2) proj. on finite-dim  $V_h$  ( $:=$  space of piecewise linear func's).
- 3) Derive basis  $(\varphi_i)_{i=1}^N$  ( $:=$  hat func's) of  $V_h$

Find  $u_h \in V_h$ .  $u_h = \sum_1^N s_i \phi_i$  solve  $A(u_h, \phi_i) = L(\phi_i)$ .  $\forall i \leq N$ . which is a linear system.

kmk: To prove the exist & unique of the formulation. we can apply Lax-Milgram's

Thm.  $\pi: V \rightarrow V_h$  is some proj. Then: we have

$$\|u - u_h\|_V \leq \sqrt{\frac{C}{\alpha}} \|u - \pi u\|_V$$

Pf: By def:  $A(u - u_h, v) = 0$ .  $\forall v \in V_h$ .

Set  $\|v\| := (A(v, v))^{\frac{1}{2}}$ .  $e = u - u_h \perp V_h$

$$\begin{aligned} \Rightarrow \|e\|^2 &= A(e, u - \pi u) + A(e, \pi u - u_h) \\ &= A(e, u - \pi u) \leq \|e\| \|u - \pi u\|. \end{aligned}$$

$$\begin{aligned} \text{So: } \|e\|_V^2 &\leq \frac{1}{\alpha} \|e\|^2 \leq \frac{1}{\alpha} \|u - \pi u\|^2 \\ &\leq \frac{C}{\alpha} \|u - \pi u\|_V^2 \end{aligned}$$

LEM.  $V := H_0^1(0, 1)$ .  $V_h := \{v \in C[0, 1] \mid v|_{[x_i, x_{i+1}]}$  is linear.  $\forall i$ .  $v(0) = v(1) = 0$ .  $x_i = ih$ .  $h = 1/n\}$ .

$\pi: V \rightarrow V_h$ .  $\pi v := \sum_1^N v(x_i) \phi_i(x)$ . where  $(\phi_i)$  is basis of  $V_h$ . Then:  $\forall v \in H_0^2(0, 1)$   
 $\Rightarrow \|v - \pi v\|_V \leq Ch \|v''\|_{L^2}$ .

Pf: It's proved in PDE I.

Pmf: Consider  $(-u(x)u'(x))' + r(x)u(x) = f(x)$   
 $u(0) = u(1) = 0.$

$\forall r \in C^1, f \in L^2$ . Then we in fact  
 can prove:  $\|u\|_{H^2} \leq \|f\|_{L^2}.$

Cor. (Aubin-Nitsche duality)

under cond. of Lem. above

$$\Rightarrow \|u - u_h\|_{L^2} \leq Ch^2 \|u\|_{H^2}.$$

Pf: Note  $\exists \varphi \in V$  s.t.  $\forall v \in V$ .

$$A(\varphi, v) = \langle \varphi, v \rangle. \text{ Since } \varphi \in H^1$$

so  $\varphi \in L^2 \Rightarrow \varphi$  is well-def.

$$\|\varphi\|_{L^2}^2 = \langle \varphi, \varphi \rangle_{L^2} = A(\varphi, \varphi)$$

$$= A(\varphi - 2\varphi, \varphi)$$

$$\leq \|\varphi\| \|\varphi - 2\varphi\|$$

By Lem. and Rank above:

$$\|\varphi - 2\varphi\| \leq Ch \|\varphi\|_{H^2} \leq Ch \|\varphi\|_{L^2}$$

$$\text{So: } \|\varphi\|_{L^2} \leq Ch \|\varphi\| \leq Ch \|\varphi\|_{H^1}$$

$$\leq Ch^2 \|u\|_{H^2}.$$

Next, we consider FEM for parabolic PDE  
 with Dirichlet boundary cond.:



$$(6.29) \quad \forall 0 < t \leq T, \forall v \in H_0^1(G) : \langle \partial_t u(t, \cdot), v \rangle_{H^{-1}(G); H_0^1(G)} + A(u, v; t) = L(v; t), \quad u(0, \cdot) = u_0.$$

Assume sol.  $u \in L^2([0, T], H_0^1(G))$  exists in the sense of  $\partial_t u \in L^2([0, T], H^{-1}(G))$ ,  $G = (0, 1)$ .

Remark: i) let  $A(u, v) = \langle u', v' \rangle_{L^2}$ ,  $L = 0 \Rightarrow$  it becomes heat equation.

ii) It's natural to assume  $\partial_t u(t, \cdot) \in H^{-1}(G)$ . Since  $\partial_t u = Au$  in i).  $\Rightarrow$   $1 - 2 = -1$  is order of  $\partial_t u$ .

For simplicity:

$$(6.28a) \quad \partial_t u(t, x) = \Delta u(t, x) + f(t, x), \quad 0 < x < 1, \quad 0 < t \leq T,$$

$$(6.28b) \quad u(0, x) = u_0(x), \quad 0 \leq x \leq 1, \quad u(t, 0) = u(t, 1) = 0, \quad 0 \leq t \leq T, \quad (6.28)$$

where  $\Delta = \partial_x^2$  only acts on the space variable  $x$ .

Thm. (Energy Dissipation)

$\exists$  const.  $k$ . Set sol.  $u$  of (6.28) satisfies:

$$\|u(t, \cdot)\|_{L^2}^2 \leq e^{-kt} \|u_0\|_{L^2}^2 + k \int_0^t e^{-k(t-s)} \|f(s, \cdot)\|_{L^2}^2 ds$$

pf: Note  $A(u(t, \cdot), u(t, \cdot))$

$$\stackrel{\text{Poincaré}}{=} \|\partial_x u(t, \cdot)\|_{L^2}^2 \geq 2 \|u(t, \cdot)\|_{L^2}^2$$

$$S_0 : \frac{1}{2} \frac{d}{dt} \|u(t, \cdot)\|_{L^2}^2 + 2 \|u(t, \cdot)\|_{L^2}^2$$

$$= -A(u(t, \cdot), u(t, \cdot)) + 2 \|u(t, \cdot)\|_{L^2}^2 + \int f u$$

$$\leq \int f u \leq \|f(t, \cdot)\|_{L^2} \|u(t, \cdot)\|_{L^2}$$

$$\leq \frac{1}{2} ( \|f(t, \cdot)\|_{L^2}^2 + \|u(t, \cdot)\|_{L^2}^2 )$$

$$\int_0^t \frac{1}{\Delta t} ( e^{kt} \|u(t, \cdot)\|_{L^2}^2 ) \leq \|f(t, \cdot)\|_{L^2}^2.$$

Next, we still consider  $h = 1/(N+1)$ .  $x_j = jh$ .

$\Delta t = \tau/m$ .  $t^m = m \Delta t$ . Denote:  $W^m := W(t^m, \cdot)$ .

Def: i)  $W^{m+\theta} := \theta W^{m+1} + (1-\theta) W^m$ .  $0 \leq m \leq M-1$ .

— ii) Consider  $u_h^m \in V_h$ .  $u_h^0 = \text{Proj}_{V_h}^{L^2} u_0$ . We

say  $(u_h^m)_{m=0}^M$  is sol. of  $\theta$ -scheme

if:  $\forall 0 \leq m \leq M-1$ .

$$\left\langle \frac{u_h^{m+1} - u_h^m}{\Delta t}, v \right\rangle_{L^2} + A(u_h^m, v) = \langle f^{m+\theta}, v \rangle_{L^2}$$

For  $\theta = 0$ . it's forward Euler approxi.

For  $\theta = 1$ . it's backward Euler approxi.

Thm. For  $1/2 \leq \theta \leq 1$ .  $\theta$ -scheme is uncond.

stable. i.e.  $\max_m \|u_h^m\|_{L^2}^2 \leq \|u_h^0\|_{L^2}^2 + \Delta t \sum_0^{M-1} \|f^{m+\theta}\|_{L^2}^2$

For  $0 \leq \theta < 1/2$ .  $\theta$ -scheme is stable if

$\exists 0 < \varepsilon < 1$ .  $\Delta t \leq h^2 (1-\varepsilon) / (6(1-2\theta))$ . Besides,

$\max_m \|u_h^m\|_{L^2}^2 \leq \|u_h^0\|_{L^2}^2 + C_\varepsilon \Delta t \sum_0^{M-1} \|f^{m+\theta}\|_{L^2}^2$ , where

$$C_\varepsilon = (4\varepsilon^2)^{-1} + \Delta t (1-2\theta) (1+\varepsilon^{-1}).$$

Pf: Only for  $\frac{1}{2} \leq \theta \leq 1$ .

Note  $u_h^{m+\theta} = \Delta t (\theta - \frac{1}{2}) \frac{u_h^{m+1} - u_h^m}{\Delta t} + \frac{u_h^m + u_h^{m+1}}{2}$

Plug it into the scheme:

$$0 \leq \Delta t (\theta - 1/2) \left\| \frac{u_h^{m+1} - u_h^m}{\Delta t} \right\|_{L^2}^2 + \frac{1}{2\Delta t} (\|u_h^{m+1}\|_{L^2}^2 - \|u_h^m\|_{L^2}^2) + \|\nabla u_h^{m+\theta}\|_{L^2}^2 = \langle f^{m+\theta}, u_h^{m+\theta} \rangle_{L^2} \leq \square + \square$$

Thm. For  $u$  is sol. of (6.28) and  $(u_h^m)_0^m$

is its backward Euler approx.:  $\forall$

$$\sup_{[0,T]} \|\partial_t u(t, \cdot)\|_{L^2} \vee \sup_{[0,T]} \|\partial_t u(t, \cdot)\|_{H^2} < \infty.$$

Then:  $\exists C > 0$  st.  $\max_{m=1, \dots, M} \|u^m - u_h^m\|_{L^2} \leq C(\Delta t + h^2)$

Pf: Denote  $\text{Proj}_h : V \rightarrow V_h$ .  $\|v\| = (A(v, v))^{1/2}$

Error Decomp.  $e_h^m := u^m - u_h^m := \eta^m + \zeta^m$

$\eta^m := u^m - P_h u^m \in V$ .  $\zeta^m = P_h u^m - u_h^m \in V_h$ .

1) By Lem. before:  $\|\eta^m\|_{L^2} \leq C h^2 \|u^m\|_{H^2}$

Similarly,  $\|\frac{\eta^{m+1} - \eta^m}{\Delta t}\|_{L^2} \leq C h^2 \|\frac{u^{m+1} - u^m}{\Delta t}\|_{H^2}$

2) Next we estimate  $\zeta^m$ :

$m=0$ . Note  $u_h^0 = \text{Proj}_{V_h} u^0$ . So:

$$\zeta_h^0 \perp_{L^2} V_h \Rightarrow \langle \zeta^0, v \rangle_{L^2} = - \langle \eta^0, v \rangle_{L^2}$$

$$\text{Let } v = \zeta^0 \in V_h \Rightarrow \|\zeta^0\|_{L^2} \leq \|\eta^0\|_{L^2} \leq C h^2 \|u^0\|_{H^2}$$

For  $1 \leq m \leq M$ . We have for  $\forall v \in V_h$ .

$$\left\langle \frac{\xi^{m+1} - \xi^m}{\Delta t}, v \right\rangle_{L^2} + A(\xi^{m+1}, v) = \left\langle \frac{u^{m+1} - u^m}{\Delta t} - \partial_t u^{m+1} - \frac{\eta^{m+1} - \eta^m}{\Delta t}, v \right\rangle_{L^2}$$

$$\stackrel{A}{=} \langle \tilde{f}^{m+1}, v \rangle_{L^2}$$

from backward Euler scheme.

By the above:

$$\max \| \tilde{f}^m \|_{L^2}^2 \leq \| f^0 \|_{L^2}^2 + \Delta t \sum_0^{m-1} \| \tilde{f}^{m+1} \|_{L^2}^2.$$

i) Estimate  $\| \tilde{f}^{m+1} \|_{L^2}^2$ :

$$\| \tilde{f}^{m+1} \|_{L^2} \leq \left\| \frac{u^{m+1} - u^m}{\Delta t} - \partial_t u^{m+1} \right\|_{L^2} + \left\| \frac{\eta^{m+1} - \eta^m}{\Delta t} \right\|_{L^2}$$

$$:= A + B.$$

$$B \stackrel{i)}{\leq} C h^2 \| \Delta t^{-1} \int_{t^m}^{t^{m+1}} \partial_t^2 u(t, \cdot) dt \|_{H^1}$$

$$\stackrel{Hölder}{\leq} C h^2 \left( \int_{t^m}^{t^{m+1}} \| \partial_t^2 u(t, \cdot) \|_{H^1}^2 dt \right)^{\frac{1}{2}} / \Delta t^{\frac{1}{2}}.$$

$$A \stackrel{Taylor}{=} \| \Delta t^{-1} \int_{t^m}^{t^{m+1}} (t - t^m) \partial_t^2 u(t, \cdot) dt \|_{L^2}$$

$$\left| \int_{t^m}^{t^{m+1}} (t - t^m) \partial_t^2 u(t, \cdot) dt \right|^2 \leq$$

$$\int_0^1 dt \int_{t^m}^{t^{m+1}} (t - t^m)^2 (\partial_t^2 u(t, \cdot))^2 dt$$

$$\leq \Delta t^2 \int_{t^m}^{t^{m+1}} (\partial_t^2 u(t, \cdot))^2 dt.$$

$$\Rightarrow A^2 \leq C \Delta t \int_{t^m}^{t^{m+1}} \| \partial_t^2 u(t, \cdot) \|_{L^2}^2 dt.$$

Remark: For  $\theta = \frac{1}{2}$ -Scheme.  $L^2$ -error =  $\Delta t^2 + h^2$